formal/fstar/ocaml-output/Tableau_CountingOracle.ml
@@ -387,8 +387,409 @@ let encode_counting_fragment (ast : counting_ast) : Prims.string=
              (Prims.strcat (ico_decls names)
                 (Prims.strcat (ico_bound_asserts inds roles fillers axs)
                    "(check-sat)\n")))))
-let z3_check_sat (smtlib : Prims.string) (rlimit : Prims.nat) : z3_verdict=
-    (* Issue #296: Phase-0 Z3_Unknown -- z3 NOT consulted yet; never
-     fabricate Z3_Unsat/Z3_Sat. See
+let ico_rdfs_subClassOf : RDF_Term.wf_iri=
+  "http://www.w3.org/2000/01/rdf-schema#subClassOf"
+let ico_owl_equivalentClass : RDF_Term.wf_iri=
+  "http://www.w3.org/2002/07/owl#equivalentClass"
+let ico_owl_someValuesFrom : RDF_Term.wf_iri=
+  "http://www.w3.org/2002/07/owl#someValuesFrom"
+let ico_owl_inverseOf : RDF_Term.wf_iri=
+  "http://www.w3.org/2002/07/owl#inverseOf"
+let ico_owl_unionOf : RDF_Term.wf_iri=
+  "http://www.w3.org/2002/07/owl#unionOf"
+let ico_owl_oneOf2 : RDF_Term.wf_iri= "http://www.w3.org/2002/07/owl#oneOf"
+let ico_owl_disjointWith : RDF_Term.wf_iri=
+  "http://www.w3.org/2002/07/owl#disjointWith"
+let ico_rdfs_domain : RDF_Term.wf_iri=
+  "http://www.w3.org/2000/01/rdf-schema#domain"
+let ico_rdfs_range : RDF_Term.wf_iri=
+  "http://www.w3.org/2000/01/rdf-schema#range"
+let ico_owl_Thing2 : RDF_Term.wf_iri= "http://www.w3.org/2002/07/owl#Thing"
+let ico_digit (c : FStar_Char.char) :
+  Prims.nat FStar_Pervasives_Native.option=
+  if c = 48
+  then FStar_Pervasives_Native.Some Prims.int_zero
+  else
+    if c = 49
+    then FStar_Pervasives_Native.Some Prims.int_one
+    else
+      if c = 50
+      then FStar_Pervasives_Native.Some (Prims.of_int (2))
+      else
+        if c = 51
+        then FStar_Pervasives_Native.Some (Prims.of_int (3))
+        else
+          if c = 52
+          then FStar_Pervasives_Native.Some (Prims.of_int (4))
+          else
+            if c = 53
+            then FStar_Pervasives_Native.Some (Prims.of_int (5))
+            else
+              if c = 54
+              then FStar_Pervasives_Native.Some (Prims.of_int (6))
+              else
+                if c = 55
+                then FStar_Pervasives_Native.Some (Prims.of_int (7))
+                else
+                  if c = 56
+                  then FStar_Pervasives_Native.Some (Prims.of_int (8))
+                  else
+                    if c = 57
+                    then FStar_Pervasives_Native.Some (Prims.of_int (9))
+                    else FStar_Pervasives_Native.None
+let rec ico_digits (acc : Prims.nat) (cs : FStar_Char.char Prims.list) :
+  Prims.nat FStar_Pervasives_Native.option=
+  match cs with
+  | [] -> FStar_Pervasives_Native.Some acc
+  | c::tl ->
+      (match ico_digit c with
+       | FStar_Pervasives_Native.None -> FStar_Pervasives_Native.None
+       | FStar_Pervasives_Native.Some d ->
+           ico_digits ((acc * (Prims.of_int (10))) + d) tl)
+let ico_parse_nat (s : Prims.string) :
+  Prims.nat FStar_Pervasives_Native.option=
+  match FStar_String.list_of_string s with
+  | [] -> FStar_Pervasives_Native.None
+  | cs -> ico_digits Prims.int_zero cs
+let rec ico_all_iris (ts : RDF_Triple.triple Prims.list) :
+  RDF_Term.wf_iri Prims.list=
+  match ts with
+  | [] -> []
+  | t::tl ->
+      FStar_List_Tot_Base.op_At
+        (match t.RDF_Triple.s with | RDF_Term.S_IRI i -> [i] | uu___ -> [])
+        (FStar_List_Tot_Base.op_At
+           (match t.RDF_Triple.o with | RDF_Term.T_IRI i -> [i] | uu___ -> [])
+           (ico_all_iris tl))
+let ico_cvar (classes : RDF_Term.wf_iri Prims.list) (c : RDF_Term.wf_iri) :
+  Prims.string=
+  Prims.strcat "c"
+    (Prims.string_of_int (ico_iri_index classes c Prims.int_zero))
+let rec ico_props_typed (ts : RDF_Triple.triple Prims.list)
+  (cls : RDF_Term.wf_iri) : RDF_Term.wf_iri Prims.list=
+  match ts with
+  | [] -> []
+  | t::tl ->
+      FStar_List_Tot_Base.op_At
+        (if
+           (t.RDF_Triple.p = ico_rdf_type) &&
+             (match t.RDF_Triple.o with
+              | RDF_Term.T_IRI i -> i = cls
+              | uu___ -> false)
+         then
+           match t.RDF_Triple.s with | RDF_Term.S_IRI i -> [i] | uu___ -> []
+         else []) (ico_props_typed tl cls)
+let rec ico_find_dom (ts : RDF_Triple.triple Prims.list)
+  (p : RDF_Term.wf_iri) : RDF_Term.wf_iri FStar_Pervasives_Native.option=
+  match ts with
+  | [] -> FStar_Pervasives_Native.None
+  | t::tl ->
+      if
+        (t.RDF_Triple.p = ico_rdfs_domain) &&
+          ((match t.RDF_Triple.s with
+            | RDF_Term.S_IRI i -> i = p
+            | uu___ -> false))
+      then
+        (match t.RDF_Triple.o with
+         | RDF_Term.T_IRI i ->
+             if i = ico_owl_Thing2
+             then ico_find_dom tl p
+             else FStar_Pervasives_Native.Some i
+         | uu___ -> ico_find_dom tl p)
+      else ico_find_dom tl p
+let rec ico_find_inv (ts : RDF_Triple.triple Prims.list)
+  (p : RDF_Term.wf_iri) : RDF_Term.wf_iri FStar_Pervasives_Native.option=
+  match ts with
+  | [] -> FStar_Pervasives_Native.None
+  | t::tl ->
+      if t.RDF_Triple.p = ico_owl_inverseOf
+      then
+        (match ((t.RDF_Triple.s), (t.RDF_Triple.o)) with
+         | (RDF_Term.S_IRI a, RDF_Term.T_IRI b) ->
+             if a = p
+             then FStar_Pervasives_Native.Some b
+             else
+               if b = p
+               then FStar_Pervasives_Native.Some a
+               else ico_find_inv tl p
+         | uu___ -> ico_find_inv tl p)
+      else ico_find_inv tl p
+let rec ico_disjoint (ts : RDF_Triple.triple Prims.list)
+  (a : RDF_Term.wf_iri) (b : RDF_Term.wf_iri) : Prims.bool=
+  match ts with
+  | [] -> false
+  | t::tl ->
+      ((t.RDF_Triple.p = ico_owl_disjointWith) &&
+         (match ((t.RDF_Triple.s), (t.RDF_Triple.o)) with
+          | (RDF_Term.S_IRI x, RDF_Term.T_IRI y) ->
+              ((x = a) && (y = b)) || ((x = b) && (y = a))
+          | uu___ -> false))
+        || (ico_disjoint tl a b)
+let rec ico_svf_via (g : RDF_Graph.rdf_graph)
+  (bs : RDF_Term.rdf_term Prims.list) (p : RDF_Term.wf_iri) :
+  RDF_Term.wf_iri FStar_Pervasives_Native.option=
+  match bs with
+  | [] -> FStar_Pervasives_Native.None
+  | b::tl ->
+      (match Tableau.term_as_subject b with
+       | FStar_Pervasives_Native.Some s ->
+           (match Tableau.find_first_object g s ico_owl_onProperty with
+            | FStar_Pervasives_Native.Some (RDF_Term.T_IRI pp) ->
+                if pp = p
+                then
+                  (match Tableau.find_first_object g s ico_owl_someValuesFrom
+                   with
+                   | FStar_Pervasives_Native.Some (RDF_Term.T_IRI x) ->
+                       FStar_Pervasives_Native.Some x
+                   | uu___ -> ico_svf_via g tl p)
+                else ico_svf_via g tl p
+            | uu___ -> ico_svf_via g tl p)
+       | FStar_Pervasives_Native.None -> ico_svf_via g tl p)
+let rec ico_exactcard_via (g : RDF_Graph.rdf_graph)
+  (bs : RDF_Term.rdf_term Prims.list) (invp : RDF_Term.wf_iri) :
+  Prims.nat FStar_Pervasives_Native.option=
+  match bs with
+  | [] -> FStar_Pervasives_Native.None
+  | b::tl ->
+      (match Tableau.term_as_subject b with
+       | FStar_Pervasives_Native.Some s ->
+           (match Tableau.find_first_object g s ico_owl_onProperty with
+            | FStar_Pervasives_Native.Some (RDF_Term.T_IRI pp) ->
+                if pp = invp
+                then
+                  (match Tableau.find_first_object g s ico_owl_cardinality
+                   with
+                   | FStar_Pervasives_Native.Some (RDF_Term.T_Literal l) ->
+                       (match ico_parse_nat l.RDF_Term.lexical_form with
+                        | FStar_Pervasives_Native.Some k ->
+                            FStar_Pervasives_Native.Some k
+                        | FStar_Pervasives_Native.None ->
+                            ico_exactcard_via g tl invp)
+                   | uu___ -> ico_exactcard_via g tl invp)
+                else ico_exactcard_via g tl invp
+            | uu___ -> ico_exactcard_via g tl invp)
+       | FStar_Pervasives_Native.None -> ico_exactcard_via g tl invp)
+let ico_restr_of (g : RDF_Graph.rdf_graph) (c : RDF_Term.wf_iri) :
+  RDF_Term.rdf_term Prims.list=
+  FStar_List_Tot_Base.op_At
+    (RDF_Graph_Executable.find_objects g (RDF_Term.S_IRI c)
+       ico_rdfs_subClassOf)
+    (RDF_Graph_Executable.find_objects g (RDF_Term.S_IRI c)
+       ico_owl_equivalentClass)
+let ico_fiber_of (g : RDF_Graph.rdf_graph)
+  (classes : RDF_Term.wf_iri Prims.list) (p : RDF_Term.wf_iri) :
+  Prims.string=
+  match ((ico_find_dom g p), (ico_find_inv g p)) with
+  | (FStar_Pervasives_Native.Some d, FStar_Pervasives_Native.Some ip) ->
+      (match ico_svf_via g (ico_restr_of g d) p with
+       | FStar_Pervasives_Native.Some x ->
+           (match ico_exactcard_via g (ico_restr_of g x) ip with
+            | FStar_Pervasives_Native.Some k ->
+                Prims.strcat "(assert (= "
+                  (Prims.strcat (ico_cvar classes d)
+                     (Prims.strcat " (* "
+                        (Prims.strcat (Prims.string_of_int k)
+                           (Prims.strcat " "
+                              (Prims.strcat (ico_cvar classes x) ")))\n")))))
+            | FStar_Pervasives_Native.None -> "")
+       | FStar_Pervasives_Native.None -> "")
+  | uu___ -> ""
+let rec ico_fiber_asserts (g : RDF_Graph.rdf_graph)
+  (classes : RDF_Term.wf_iri Prims.list) (ps : RDF_Term.wf_iri Prims.list) :
+  Prims.string=
+  match ps with
+  | [] -> ""
+  | p::tl ->
+      Prims.strcat (ico_fiber_of g classes p)
+        (ico_fiber_asserts g classes tl)
+let rec ico_bij_for_prop (g : RDF_Graph.rdf_graph)
+  (classes : RDF_Term.wf_iri Prims.list) (p : RDF_Term.wf_iri)
+  (ip : RDF_Term.wf_iri) (cs : RDF_Term.wf_iri Prims.list) : Prims.string=
+  match cs with
+  | [] -> ""
+  | d::tl ->
+      let this =
+        match ico_svf_via g (ico_restr_of g d) p with
+        | FStar_Pervasives_Native.Some y ->
+            (match ico_svf_via g (ico_restr_of g y) ip with
+             | FStar_Pervasives_Native.Some dback ->
+                 if dback = d
+                 then
+                   Prims.strcat "(assert (= "
+                     (Prims.strcat (ico_cvar classes d)
+                        (Prims.strcat " "
+                           (Prims.strcat (ico_cvar classes y) "))\n")))
+                 else ""
+             | FStar_Pervasives_Native.None -> "")
+        | FStar_Pervasives_Native.None -> "" in
+      Prims.strcat this (ico_bij_for_prop g classes p ip tl)
+let rec ico_bij_asserts (g : RDF_Graph.rdf_graph)
+  (classes : RDF_Term.wf_iri Prims.list) (ps : RDF_Term.wf_iri Prims.list) :
+  Prims.string=
+  match ps with
+  | [] -> ""
+  | p::tl ->
+      Prims.strcat
+        (match ico_find_inv g p with
+         | FStar_Pervasives_Native.Some ip ->
+             ico_bij_for_prop g classes p ip classes
+         | FStar_Pervasives_Native.None -> "") (ico_bij_asserts g classes tl)
+let ico_union_of_triple (g : RDF_Graph.rdf_graph)
+  (classes : RDF_Term.wf_iri Prims.list) (t : RDF_Triple.triple) :
+  Prims.string=
+  if t.RDF_Triple.p = ico_owl_equivalentClass
+  then
+    match ((t.RDF_Triple.s), (t.RDF_Triple.o)) with
+    | (RDF_Term.S_IRI z, RDF_Term.T_BNode uu___) ->
+        (match Tableau.term_as_subject t.RDF_Triple.o with
+         | FStar_Pervasives_Native.Some bs ->
+             (match Tableau.find_first_object g bs ico_owl_unionOf with
+              | FStar_Pervasives_Native.Some lterm ->
+                  (match Tableau.walk_rdf_list g lterm
+                           (FStar_List_Tot_Base.length g)
+                   with
+                   | (RDF_Term.T_IRI m1)::(RDF_Term.T_IRI m2)::[] ->
+                       if ico_disjoint g m1 m2
+                       then
+                         Prims.strcat "(assert (= "
+                           (Prims.strcat (ico_cvar classes z)
+                              (Prims.strcat " (+ "
+                                 (Prims.strcat (ico_cvar classes m1)
+                                    (Prims.strcat " "
+                                       (Prims.strcat (ico_cvar classes m2)
+                                          ")))\n")))))
+                       else ""
+                   | uu___1 -> "")
+              | FStar_Pervasives_Native.None -> "")
+         | FStar_Pervasives_Native.None -> "")
+    | uu___ -> ""
+  else ""
+let rec ico_union_asserts (g : RDF_Graph.rdf_graph)
+  (classes : RDF_Term.wf_iri Prims.list) (ts : RDF_Triple.triple Prims.list)
+  : Prims.string=
+  match ts with
+  | [] -> ""
+  | t::tl ->
+      Prims.strcat (ico_union_of_triple g classes t)
+        (ico_union_asserts g classes tl)
+let ico_list_nonempty (g : RDF_Graph.rdf_graph) (head : RDF_Term.rdf_term) :
+  Prims.bool=
+  match Tableau.term_as_subject head with
+  | FStar_Pervasives_Native.Some s ->
+      (match Tableau.find_first_object g s OWL_Closure.rdf_first with
+       | FStar_Pervasives_Native.Some uu___ -> true
+       | FStar_Pervasives_Native.None -> false)
+  | FStar_Pervasives_Native.None -> false
+let rec ico_any_equiv_oneof (g : RDF_Graph.rdf_graph)
+  (bs : RDF_Term.rdf_term Prims.list) : Prims.bool=
+  match bs with
+  | [] -> false
+  | b::tl ->
+      (match Tableau.term_as_subject b with
+       | FStar_Pervasives_Native.Some s ->
+           (match Tableau.find_first_object g s ico_owl_oneOf2 with
+            | FStar_Pervasives_Native.Some l -> ico_list_nonempty g l
+            | FStar_Pervasives_Native.None -> false)
+       | FStar_Pervasives_Native.None -> false) || (ico_any_equiv_oneof g tl)
+let ico_class_has_oneof (g : RDF_Graph.rdf_graph) (c : RDF_Term.wf_iri) :
+  Prims.bool=
+  (match Tableau.find_first_object g (RDF_Term.S_IRI c) ico_owl_oneOf2 with
+   | FStar_Pervasives_Native.Some l -> ico_list_nonempty g l
+   | FStar_Pervasives_Native.None -> false) ||
+    (ico_any_equiv_oneof g
+       (RDF_Graph_Executable.find_objects g (RDF_Term.S_IRI c)
+          ico_owl_equivalentClass))
+let rec ico_oneof_asserts (g : RDF_Graph.rdf_graph)
+  (classes : RDF_Term.wf_iri Prims.list) (cs : RDF_Term.wf_iri Prims.list) :
+  Prims.string=
+  match cs with
+  | [] -> ""
+  | c::tl ->
+      Prims.strcat
+        (if ico_class_has_oneof g c
+         then
+           Prims.strcat "(assert (>= "
+             (Prims.strcat (ico_cvar classes c) " 1))\n")
+         else "") (ico_oneof_asserts g classes tl)
+let rec ico_class_decls (classes : RDF_Term.wf_iri Prims.list)
+  (cs : RDF_Term.wf_iri Prims.list) : Prims.string=
+  match cs with
+  | [] -> ""
+  | c::tl ->
+      Prims.strcat "(declare-const "
+        (Prims.strcat (ico_cvar classes c)
+           (Prims.strcat " Int)\n"
+              (Prims.strcat "(assert (>= "
+                 (Prims.strcat (ico_cvar classes c)
+                    (Prims.strcat " 0))\n" (ico_class_decls classes tl))))))
+let rec ico_iri_inter (xs : RDF_Term.wf_iri Prims.list)
+  (ys : RDF_Term.wf_iri Prims.list) : RDF_Term.wf_iri Prims.list=
+  match xs with
+  | [] -> []
+  | h::tl ->
+      FStar_List_Tot_Base.op_At (if ico_mem_iri h ys then [h] else [])
+        (ico_iri_inter tl ys)
+let encode_counting_smt (g : RDF_Graph.rdf_graph) : Prims.string=
+  let classes = ico_dedup_iri (ico_all_iris g) in
+  let fprops = ico_props_typed g ico_owl_FunctionalProperty in
+  let ifprops = ico_props_typed g ico_owl_InverseFunctionalProperty in
+  let bprops = ico_iri_inter fprops ifprops in
+  Prims.strcat "(set-logic QF_LIA)\n"
+    (Prims.strcat "; Z33kr counting-fragment class-size encoding (Phase 1)\n"
+       (Prims.strcat (ico_class_decls classes classes)
+          (Prims.strcat (ico_fiber_asserts g classes fprops)
+             (Prims.strcat (ico_bij_asserts g classes bprops)
+                (Prims.strcat (ico_union_asserts g classes g)
+                   (Prims.strcat (ico_oneof_asserts g classes classes)
+                      "(check-sat)\n"))))))
+let z3_check_sat smtlib rlimit =
+  (* Issue #296: Phase-1 native z3 spawn (ASSUME-HOST + ASSUME-IO).
+     Realisation ONLY -- satisfiability is z3's semantics; the counting
+     encoding is the verified F* Tot function encode_counting_smt. Any
+     failure => Z3_Unknown, NEVER a fabricated verdict. See
      minimal_regrettable_glue_code_each_with_an_open_issue/296_z3_check_sat.sh *)
-  Z3_Unknown
+  (try Sys.set_signal Sys.sigpipe Sys.Signal_ignore with _ -> ());
+  (try
+     let z3bin = (try Sys.getenv "FACTOIDAL_Z3_BIN" with Not_found -> "z3") in
+     (* NB: the extracted module opens Prims, so a bare `>` / `*` are the
+        Z.t operators. Use Z.gt / Z.zero explicitly and keep rl as a
+        Stdlib int only for Printf's %d. *)
+     let rl = (try Z.to_int rlimit with _ -> 0) in
+     let use_rlimit = (try Z.gt rlimit Z.zero with _ -> false) in
+     let smt =
+       (if use_rlimit then Printf.sprintf "(set-option :rlimit %d)\n" rl else "")
+       ^ smtlib in
+     (* child stdout -> parent reads r_out; parent writes w_in -> child stdin *)
+     (* cloexec on BOTH pipes: create_process dup2s r_in/w_out onto the
+        child's fd0/fd1 (clearing cloexec on those dups), then exec closes
+        every remaining cloexec fd -- so the child does NOT inherit the
+        parent's write-end of its stdin (w_in). Without this the child
+        keeps w_in open, its stdin never reaches EOF, z3 blocks forever,
+        and the read below deadlocks (the wall-clock cap then reports it
+        as Unknown). *)
+     let (r_out, w_out) = Unix.pipe ~cloexec:true () in
+     let (r_in, w_in) = Unix.pipe ~cloexec:true () in
+     let pid =
+       Unix.create_process z3bin [| z3bin; "-in"; "-smt2" |] r_in w_out Unix.stderr in
+     Unix.close r_in; Unix.close w_out;
+     let oc = Unix.out_channel_of_descr w_in in
+     (try output_string oc smt; flush oc with _ -> ());
+     (try close_out oc with _ -> ());
+     let ic = Unix.in_channel_of_descr r_out in
+     let rec read_lines acc =
+       match (try Some (input_line ic) with End_of_file -> None) with
+       | Some l -> read_lines (l :: acc)
+       | None -> List.rev acc in
+     let lines = read_lines [] in
+     (try close_in ic with _ -> ());
+     (try ignore (Unix.waitpid [] pid) with _ -> ());
+     let rec first = function
+       | [] -> Z3_Unknown
+       | l :: tl ->
+         (match String.trim l with
+          | "unsat" -> Z3_Unsat
+          | "sat" -> Z3_Sat
+          | "unknown" -> Z3_Unknown
+          | _ -> first tl) in
+     first lines
+   with _ -> Z3_Unknown)
